Soundness wip

typing.v
@@ -1,4 +1,5 @@
-Require Export syntax.
+Require Export syntax ssrbool ssreflect.
+From Hammer Require Import Tactics.
 
 Definition context n := fin n -> ty.
 
@@ -18,10 +19,6 @@ Inductive Wt {n} (Γ : context n) : tm n -> ty -> Prop :=
   Γ ⊢ a ∈ A ->
   (* -------------- *)
   Γ ⊢ App b a ∈ B
-
-| T_K :
-  (* --------- *)
-  Γ ⊢ TmK ∈ TyK
 
 | T_Unit :
   (* ------------- *)
@@ -48,18 +45,90 @@ Inductive DEquiv {n} (Γ : context n) : tm n -> tm n -> ty -> Prop :=
   (* -------------  *)
   Γ ⊢ Lam A b0 ≡ Lam A b1 ∈ Fun A B
 | DE_App b0 b1 a0 a1 A B :
+  Γ ⊢ b0 ≡ b1 ∈ Fun A B ->
+  Γ ⊢ a0 ≡ a1 ∈ A ->
+  (*--------------------  *)
+  Γ ⊢ App b0 a0 ≡ App b1 a1 ∈ B
+| DE_AppAbs b0 b1 a0 a1 A B :
   A.:Γ ⊢ b0 ≡ b1 ∈ B ->
   Γ ⊢ a0 ≡ a1 ∈ A ->
   (* ---------------- *)
   Γ ⊢ App (Lam A b0) a0 ≡ subst_tm (a1..) b1 ∈ B
-| DE_Ext b0 b1 A B :
-  A.:Γ ⊢ App (ren_tm shift b0) (var_tm var_zero) ≡
-    App (ren_tm shift b1) (var_tm var_zero) ∈ B ->
-  (* ------------------ *)
-  Γ ⊢ b0 ≡ b1 ∈ Fun A B
 | DE_Unit a b :
   Γ ⊢ a ∈ TyUnit ->
   Γ ⊢ b ∈ TyUnit ->
   (* --------------- *)
   Γ ⊢ a ≡ b ∈ TyUnit
 where "Γ ⊢ a ≡ b ∈ A" := (DEquiv Γ a b A).
+
+Definition whnf {n} (a : tm n) :=
+  match a with
+  | TmUnit => true
+  | Lam _ _ => true
+  | _ => false
+  end.
+
+Reserved Notation "Γ ⊢ a ⤳ b ∈ A" (at level 70).
+Inductive Red {n} (Γ : context n) : tm n -> tm n -> ty -> Prop :=
+(* R_App and R_AppAbs don't overlap because Abs can't be reduced *)
+| R_App b0 b1 a A B :
+  Γ ⊢ b0 ⤳ b1 ∈ Fun A B ->
+  Γ ⊢ a ∈ A ->
+  (* ---------------- *)
+  Γ ⊢ App b0 a ⤳ App b1 a ∈ B
+| R_AppAbs b a A B :
+  A.:Γ ⊢ b ∈ B ->
+  Γ ⊢ a ∈ A ->
+  (* ---------------- *)
+  Γ ⊢ App (Lam A b) a ⤳ subst_tm (a..) b ∈ B
+where "Γ ⊢ a ⤳ b ∈ A" := (Red Γ a b A).
+
+Reserved Notation "Γ ⊢ a ⤳* b ∈ A" (at level 70, no associativity).
+Inductive Reds {n} (Γ : context n) (a : tm n) : tm n -> ty -> Prop :=
+| Rs_Refl A :
+  Γ ⊢ a ∈ A ->
+  Γ ⊢ a ⤳* a ∈ A
+| Rs_Step b c A :
+  Γ ⊢ a ⤳ b ∈ A ->
+  Γ ⊢ b ∈ A ->
+  Γ ⊢ b ⤳* c ∈ A ->
+  Γ ⊢ a ⤳* c ∈ A
+where "Γ ⊢ a ⤳* b ∈ A" := (Reds Γ a b A).
+
+Definition ren_ok {n m} ξ (Γ : context n) (Δ : context m) :=
+  forall i, Γ i = Δ (ξ i).
+
+Fixpoint LR {n} (Γ : context n) (b0 b1 : tm n) (A : ty) : Prop :=
+  match A with
+  | TyUnit => Γ ⊢ b0 ∈ TyUnit /\ Γ ⊢ b1 ∈ TyUnit
+  | Fun A B => Γ ⊢ b0 ≡ b1 ∈ Fun A B /\
+                forall m ξ (Δ : context m), ren_ok ξ Γ Δ ->
+                         forall a0 a1, LR Δ a0 a1 A -> LR Δ (App (ren_tm ξ b0) a0) (App (ren_tm ξ b1) a1) B
+  | _ => Γ ⊢ b0 ≡ b1 ∈ A
+  end.
+
+Lemma escape {n} (Γ : context n) (a b : tm n) (A : ty) :
+  LR Γ a b A -> Γ ⊢ a ≡ b ∈ A.
+Proof.
+  elim : A n Γ a b=> //=; hauto lq:on ctrs:DEquiv.
+Qed.
+
+Definition subst_ok {n m}
+  (ρ δ : fin n -> tm m)
+  (Γ : context n)
+  (Δ : context m) :=
+  forall i, LR Δ (ρ i) (δ i) (Γ i).
+
+Definition SEquiv {n} (Γ : context n) (b0 b1 : tm n) (A : ty) :=
+  forall m ρ δ (Δ : context m), subst_ok ρ δ Γ Δ ->
+                              LR Δ (subst_tm ρ b0) (subst_tm ρ b1) A.
+
+Notation "Γ ⊨ b0 ≡ b1 ∈ A" := (SEquiv Γ b0 b1 A) (at level 70, no associativity).
+
+Lemma soundness {n} (Γ : context n) a A : Γ ⊢ a ∈ A -> Γ ⊨ a ≡ a ∈ A.
+Proof.
+  move => h.
+  elim : n Γ a A / h.
+  - rewrite /SEquiv.
+    simpl.
+Admitted.
